Add Sims.percolate to apply a Sims.filter.

B1_finite_map.v
@@ -30,42 +30,50 @@ Section Unbalanced_binary_tree.
 
 Variable V : Type.
 
-Inductive fmap := Leaf | Node (vO : option V) (f0 f1 : fmap).
+Inductive fmap := Leaf | Node (val : option V) (fO fI : fmap).
 
 (***
 Insert and lookup mappings
 *)
 
-(* Create a map that only maps i to j. *)
-Fixpoint create (i : positive) (v : V) :=
-  match i with
-  | xH => Node (Some v) Leaf Leaf
-  | xO i' => Node None (create i' v) Leaf
-  | xI i' => Node None Leaf (create i' v)
+(* Create a map that only maps key to val. *)
+Fixpoint create (key : positive) (val : V) :=
+  match key with
+  | xH => Node (Some val) Leaf Leaf
+  | xO k => Node None (create k val) Leaf
+  | xI k => Node None Leaf (create k val)
   end.
 
-(* Insert j at i. *)
-Fixpoint insert (f : fmap) (i : positive) (v : V) :=
+(* Insert val at key. *)
+Fixpoint insert (f : fmap) (key : positive) (val : V) :=
   match f with
-  | Leaf => create i v
-  | Node vO f0 f1 =>
-    match i with
-    | xH => Node (Some v) f0 f1
-    | xO i' => Node vO (insert f0 i' v) f1
-    | xI i' => Node vO f0 (insert f1 i' v)
+  | Leaf => create key val
+  | Node v fO fI =>
+    match key with
+    | xH => Node (Some val) fO fI
+    | xO k => Node v (insert fO k val) fI
+    | xI k => Node v fO (insert fI k val)
     end
   end.
 
-(* Get the value at i. *)
-Fixpoint lookup (f : fmap) (i : positive) :=
+(* Get the value at key. *)
+Fixpoint lookup (f : fmap) (key : positive) :=
   match f with
   | Leaf => None
-  | Node vO f0 f1 =>
-    match i with
-    | xH => vO
-    | xO i' => lookup f0 i'
-    | xI i' => lookup f1 i'
+  | Node val fO fI =>
+    match key with
+    | xH => val
+    | xO k => lookup fO k
+    | xI k => lookup fI k
     end
+  end.
+
+(* Retrieve all values. *)
+Fixpoint values (f : fmap) :=
+  match f with
+  | Leaf => []
+  | Node None fO fI => values fO ++ values fI
+  | Node (Some v) fO fI => v :: values fO ++ values fI
   end.
 
 End Unbalanced_binary_tree.
@@ -75,6 +83,7 @@ Arguments Node {_}.
 Arguments create {_}.
 Arguments insert {_}.
 Arguments lookup {_}.
+Arguments values {_}.
 
 Notation ffun := (fmap positive).
 
@@ -98,23 +107,23 @@ Function composition
 Fixpoint map_ffun (g f : ffun) :=
   match f with
   | Leaf => Leaf
-  | Node (Some i) f0 f1 => Node (Some g⋅i) (map_ffun g f0) (map_ffun g f1)
-  | Node None f0 f1 => Node None (map_ffun g f0) (map_ffun g f1)
+  | Node (Some i) fO fI => Node (Some g⋅i) (map_ffun g fO) (map_ffun g fI)
+  | Node None fO fI => Node None (map_ffun g fO) (map_ffun g fI)
   end.
 
 (* Apply g after f. The initial input for g must be copied as gI. *)
 Fixpoint compose (gI g f : ffun) {struct f} :=
   match f with
   | Leaf => g
-  | Node (Some i) f0 f1 =>
+  | Node (Some i) fO fI =>
     match g with
-    | Leaf => Node (Some gI⋅i) (map_ffun gI f0) (map_ffun gI f1)
-    | Node jO g0 g1 => Node (Some gI⋅i) (compose gI g0 f0) (compose gI g1 f1)
+    | Leaf => Node (Some gI⋅i) (map_ffun gI fO) (map_ffun gI fI)
+    | Node jO g0 g1 => Node (Some gI⋅i) (compose gI g0 fO) (compose gI g1 fI)
     end
-  | Node None f0 f1 =>
+  | Node None fO fI =>
     match g with
-    | Leaf => Node None (map_ffun gI f0) (map_ffun gI f1)
-    | Node jO g0 g1 => Node jO (compose gI g0 f0) (compose gI g1 f1)
+    | Leaf => Node None (map_ffun gI fO) (map_ffun gI fI)
+    | Node jO g0 g1 => Node jO (compose gI g0 fO) (compose gI g1 fI)
     end
   end.
 
@@ -128,10 +137,10 @@ Function inversion
 Fixpoint invert (f f_inv : ffun) (r : positive) :=
   match f with
   | Leaf => f_inv
-  | Node iO f0 f1 =>
-    let f_inv' := invert f0 f_inv r~0 in
-    let f_inv'' := invert f1 f_inv' r~1 in
-    match iO with
+  | Node i_opt fO fI =>
+    let f_inv' := invert fO f_inv r~0 in
+    let f_inv'' := invert fI f_inv' r~1 in
+    match i_opt with
     | Some i => insert f_inv'' i (mirror r)
     | None => f_inv''
     end
@@ -161,10 +170,10 @@ practice if this sifting procedure actually provides a net speed-up.
 Fixpoint Pruned (f : ffun) (r : positive) :=
   match f with
   | Leaf => True
-  | Node iO f0 f1 =>
-    Pruned f0 r~0 /\
-    Pruned f1 r~1 /\
-    match iO with
+  | Node i_opt fO fI =>
+    Pruned fO r~0 /\
+    Pruned fI r~1 /\
+    match i_opt with
     | Some i => i ≠ mirror r
     | None => True
     end
@@ -172,24 +181,24 @@ Fixpoint Pruned (f : ffun) (r : positive) :=
 
 (* Remove the mappings in f that are also in s. *)
 Fixpoint sift (f s : ffun) :=
-  let collapse := λ (f0 f1 : ffun),
-    match f0, f1 with
+  let collapse := λ (fO fI : ffun),
+    match fO, fI with
     | Leaf, Leaf => Leaf
-    | f0', f1' => Node None f0' f1'
+    | fO', fI' => Node None fO' fI'
     end
   in match s with
   | Leaf => f
-  | Node iO s0 s1 =>
+  | Node i_opt s0 s1 =>
     match f with
     | Leaf => Leaf
-    | Node None f0 f1 => collapse (sift f0 s0) (sift f1 s1)
-    | Node (Some j) f0 f1 =>
-      match iO with
+    | Node None fO fI => collapse (sift fO s0) (sift fI s1)
+    | Node (Some j) fO fI =>
+      match i_opt with
       | Some i =>
         if i =? j
-        then collapse (sift f0 s0) (sift f1 s1)
-        else Node (Some j) (sift f0 s0) (sift f1 s1)
-      | None => Node (Some j) (sift f0 s0) (sift f1 s1)
+        then collapse (sift fO s0) (sift fI s1)
+        else Node (Some j) (sift fO s0) (sift fI s1)
+      | None => Node (Some j) (sift fO s0) (sift fI s1)
       end
     end
   end.
@@ -199,7 +208,7 @@ Theorems
 *)
 
 Local Ltac fmap_induction f :=
-  induction f as [|jO f0 IHf0 f1 IHf1]; simpl; intros.
+  induction f as [|j_opt fO IHfO fI IHfI]; simpl; intros.
 
 Lemma lookup_create_eq {V} i (v : V) : lookup (create i v) i = Some v.
 Proof. induction i; easy. Qed.
@@ -225,8 +234,8 @@ Proof.
 revert i j; fmap_induction f.
 apply lookup_create_neq, H.
 destruct i, j; simpl; try easy.
-apply IHf1; congruence.
-apply IHf0; congruence.
+apply IHfI; congruence.
+apply IHfO; congruence.
 Qed.
 
 Theorem lookup_insert {V} f i j (v : V) :
@@ -240,33 +249,33 @@ Lemma lookup_map_ffun_None g f i :
   lookup f i = None -> lookup (map_ffun g f) i = None.
 Proof.
 revert i; fmap_induction f. easy.
-destruct i, jO as [j|]; simpl; try easy.
-all: try apply IHf0; try apply IHf1; easy.
+destruct i, j_opt as [j|]; simpl; try easy.
+all: try apply IHfO; try apply IHfI; easy.
 Qed.
 
 Lemma lookup_compose_None gI g f i :
   lookup f i = None -> lookup (compose gI g f) i = lookup g i.
 Proof.
 revert g i; fmap_induction f. easy.
-destruct jO as [j|], g, i; simpl; try easy.
+destruct j_opt as [j|], g, i; simpl; try easy.
 1,2,5,6: apply lookup_map_ffun_None, H.
-all: try rewrite IHf1; try rewrite IHf0; easy.
+all: try rewrite IHfI; try rewrite IHfO; easy.
 Qed.
 
 Lemma lookup_map_ffun_Some g f i j :
   lookup f i = Some j -> lookup (map_ffun g f) i = Some g⋅j.
 Proof.
 revert g i; fmap_induction f. easy.
-destruct jO as [j'|], i; simpl; try congruence.
-all: try apply IHf0; try apply IHf1; easy.
+destruct j_opt as [j'|], i; simpl; try congruence.
+all: try apply IHfO; try apply IHfI; easy.
 Qed.
 
 Lemma lookup_compose_Some gI g f i j :
   lookup f i = Some j -> lookup (compose gI g f) i = Some gI⋅j.
 Proof.
 revert g i; fmap_induction f. easy.
-destruct jO as [j'|], g, i; simpl; try congruence.
-all: try apply lookup_map_ffun_Some; try apply IHf0; try apply IHf1; easy.
+destruct j_opt as [j'|], g, i; simpl; try congruence.
+all: try apply lookup_map_ffun_Some; try apply IHfO; try apply IHfI; easy.
 Qed.
 
 Theorem apply_compose g f i :
