C1_Schreier_vector.v
@@ -8,46 +8,50 @@ Definition vector := fmap perm.
 
 Section Algorithm.
 
-Fixpoint extend (i : positive) (π : perm)
+(* Add all numbers reachable from i. *)
+Fixpoint extend (i : positive) (h : perm)
   (gen : list perm) (V : vector)
   (acc : list positive) :=
   match gen with
   | [] => (V, acc)
-  | σ :: gen' =>
-    let j := σ⋅i in
+  | g :: gen' =>
+    let j := g⋅i in
     match lookup V j with
-    | Some _ => extend i π gen' V acc
-    | None => extend i π gen' (insert V j (σ ∘ π)) (j :: acc)
+    | Some _ => extend i h gen' V acc
+    | None => extend i h gen' (insert V j (g ∘ h)) (j :: acc)
     end
   end.
 
 Variable generator : list perm.
 
-Fixpoint step (V : vector) (try acc : list positive) :=
+(* Extend all numbers in the try list. *)
+Fixpoint extend_loop (V : vector) (try acc : list positive) :=
   match try with
   | [] => (V, acc)
   | i :: try' =>
     match lookup V i with
-    | Some π =>
-      match extend i π generator V acc with
-      | (V', acc') => step V' try' acc'
+    | None => extend_loop V try' acc
+    | Some h =>
+      match extend i h generator V acc with
+      | (V', acc') => extend_loop V' try' acc'
       end
-    | None => step V try' acc
     end
   end.
 
+(* Repeat orbit extension n times. *)
 Fixpoint loop (V : vector) (try : list positive) (n : nat) :=
   match n with
   | O => V
   | S m =>
-    match step V try [] with
+    match extend_loop V try [] with
     | (V', []) => V'
     | (V', try') => loop V' try' m
     end
   end.
 
-Definition build (range k : positive) :=
-  loop (insert Leaf k ident) [k] (Pos.to_nat range).
+(* Build a full orbit vector for a given permutation range. *)
+Definition build (range : nat) (k : positive) :=
+  loop (insert Leaf k ident) [k] range.
 
 End Algorithm.
 
