C2_Sims_filter.v
@@ -1,1 +1,61 @@
 (* A functional Sims-filter to reduce generator sets. *)
+
+From permutation_solver Require Import A_setup B1_finite_map B2_permutation.
+
+Module Sims.
+
+Definition filter := fmap (fmap perm).
+
+Section Algorithm.
+
+(* Find the smallest mapping in π. *)
+Fixpoint min (π : perm) : option (positive × positive) :=
+  match π with
+  | Leaf => None
+  | Node (Some j) _ _ => Some (xH, j)
+  | Node None πO πI =>
+    match min πO, min πI with
+    | None, None => None
+    | None, Some (i, j) => Some (i~0, j)
+    | Some (i, j), None => Some (i~1, j)
+    | Some (i, j), Some (i', j') =>
+      Some (if i <? i' then (i~0, j) else (i'~1, j'))
+    end
+  end.
+
+Variable sieve : perm.
+
+(* Add g to the filter or discard it. *)
+Fixpoint crack (F : filter) (range : nat) (g : perm) :=
+  match range with
+  | O => F
+  | S ran =>
+    let g' := sift g sieve in
+    match min g' with
+    | None => F
+    | Some (i, j) =>
+      match lookup F i with
+      | None => insert F i (create j g')
+      | Some Fi =>
+        match lookup Fi j with
+        | None => insert F i (insert Fi j g')
+        | Some h => crack F ran (inv g ∘ h)
+        end
+      end
+    end
+  end.
+
+Variable range : nat.
+
+Fixpoint loop (gen : list perm) (F : filter) :=
+  match gen with
+  | [] => F
+  | g :: gen' => loop gen' (crack F range g)
+  end.
+
+Definition percolate (gen : list perm) :=
+  flat_map values (values (loop gen Leaf)).
+
+End Algorithm.
+
+End Sims.
